$$: : \left[ \left( 2 b \right) 2 + \left( \frac { 3 \sqrt { 2 } } { b } \right) ^ { 2 } \right] + \left[ \left( 2 b - b \right) 2 + \left( \frac { 6 \sqrt { 2 } } { b } - \frac { 3 \sqrt { 2 } } { b } \right) ^ { 2 } \right] = b ^ { 2 } + \left( \frac { 6 \sqrt { 2 } } { b } \right) ^ { 2 } ,$$
$$: b = \sqrt { 3 }$$
$$: . B \left( \sqrt { 3 } , 2 \sqrt { 6 } \right) , D \left( 2 \sqrt { 3 } , \sqrt { 6 } \right) ,$$

: $y = 2 \sqrt { 2 } x ,$ $y = 2 \sqrt { 2 } x - 3 \sqrt { 6 } ,$ 当 $y = 0$ 时,2√2x-3√6=0,

$$x = \frac { 3 \sqrt { 3 } } { 2 }$$
$$: : F \left( \frac { 3 \sqrt { 3 } } { 2 } , 0 \right)$$
$$\cdot O E = \sqrt { 3 } , O F = \frac { 3 \sqrt { 3 } } { 2 }$$
$$: : E F = O F - O E = \frac { \sqrt { 3 } } { 2 }$$
$$: \frac { E F } { O E } = \frac { 1 } { 2 } ,$$

$\frac { 1 } { 2 } , \left( \frac { 3 \sqrt { 3 } } { 2 } , 0 \right)$ .

17.(1)计算: $\left( x + 1 \right) \left( x \quad - \quad 1 \right) + x \left( 2 \quad - \quad x \right)$ .(2)解不等式组: $\left\{ \begin{array}{} 4 x - 3 > 9 \\ 2 + x \geq 0 \end{array} \right.$

[答案]:【小问1详解】解:原式 $= x ^ { 2 } - 1 + 2 x - x ^ { 2 } = 2 x - 1$ 【小问2详解】解: $\left\{ \begin{array}{} { 4 x - 3 > 9 \left( 1 \right) } \\ { 2 + x \geq 0 \left( 2 \right) } \end{array} \right.$ ,解

不等式(1),得x>3,解不等式(2),得x≥-2,所以原不等式组的解是x>3.[解析]:

18\. 

![$$B$$ $$A$$](figures/1.1)


![$$B$$ $$A$$](figures/1.2)


![$$B$$ $$A$$ $${ } ^ { \sharp } C$$](figures/1.3)


$$B$$

$$A$$

$$C$$

![$$B$$ $$A$$ $$D$$ $$E$$](figures/1.4)


[解析]:

19\. 

![](figures/1.5)
```