<!-- PageHeader="参考答案 第85天" -->

$$4 \frac { 3 } { 5 } - 1 \frac { 1 } { 2 } = 3 \frac { 1 } { 1 0 }$$
$$6 . 6 \times 3 0 0 = 1 9 8 0$$

$$5 \frac { 1 } { 2 } - 2 \frac { 4 } { 9 } = 3 \frac { 1 } { 1 8 }$$

$$2 4 \div 1 . 2 = 2 0$$

$$4 7 . 9 5 + 2 2 . 9 5 - 3 7 . 3 5 = 3 3 . 5 5 \quad 0 . 3 \times 0 . 8 = 0 . 2 4$$

$$4 . 2 \times 2 0 = 8 4$$

$$2 0 . 3 5 + 3 . 1 8 - 1 8 . 9 2 = 4 . 6 1$$

$$8 . 0 1 \div 0 . 9 = 8 . 9$$

$$1 . 6 \times 0 . 3 = 0 . 4 8$$

$$5 + 2 . 7 - 0 . 3 = 7 . 4$$

$$9 . 3 \times 6 0 = 5 5 8$$

$$\frac { 1 } { 6 } + \frac { 3 } { 5 } = \frac { 2 3 } { 3 0 }$$

$$2 . 3 \times 5 = 1 1 . 5$$
